U: EC

code/experimental/pkcs/Hacl.Impl.PKCS11.Internal.Attribute.fst
@@ -4,7 +4,6 @@ open Lib.IntTypes
 open Hacl.Impl.PKCS11.Internal.Types
 
 open Hacl.Impl.PKCS11.Result
-open Hacl.Impl.PKCS11.External.DER
 
 open FStar.HyperStack.All
 open FStar.HyperStack
@@ -45,6 +44,7 @@ let lenAttribute attrType =
   match a with 
   |0ul -> (size 1) 
   |1ul -> (size 1)
+    (* actually, the max possible length for DER encoding? *)
   |180ul -> (size 16)
   |_ -> (size 1)
 
@@ -93,26 +93,4 @@ let isAttributeReadOnlyBuffer a b =
   let newException = exceptionAdd oldException e in 
   upd b (size 0) newException
 
-
-(* This piece of code should be in the mechanism functionality *)
-val isAttributeEC_PARAMCorrect: a: attribute {CKA_EC_PARAMS? a} -> Stack (((e: exception_t) & (_HACL_Curve_ID)))
-  (requires fun h -> True)
-  (ensures fun h0 _ h1 -> True)
-
-let isAttributeEC_PARAMCorrect a = 
-  let ulCount = CKA_EC_PARAMS?.ulValueLen a in 
-  parseEC_ANSI_962 (CKA_EC_PARAMS?.ulValueLen a) (CKA_EC_PARAMS?.pValue a)
-
-
-val checkAttributes: ulCount: size_t -> pTemplate: buffer attribute{length pTemplate = uint_v ulCount} -> Stack unit
-  (requires fun h -> live h pTemplate)
-  (ensures fun h0 _ h1 -> True)
-
-let checkAttributes ulCount pTemplate = 
-  push_frame();
-  [@inline_let]
-  let okException = CKR_OK in 
-  let bTest = LowStar.Buffer.alloca okException (normalize_term 1ul) in  
-  C.Loops.for 0ul ulCount (fun h i -> True) (fun i ->  isAttributeReadOnlyBuffer (index pTemplate i) bTest);
-  pop_frame()
 
