code/experimental/pkcs/Hacl.Impl.PKCS11.AttributeVerific.fst
@@ -1,0 +1,47 @@
+module Hacl.Impl.PKCS11.AttributeVerific
+
+open Lib.IntTypes
+open Hacl.Impl.PKCS11.Internal.Types
+
+open Hacl.Impl.PKCS11.Result
+open Hacl.Impl.PKCS11.External.DER
+
+open Hacl.Impl.PKCS11.Internal.Attribute
+open Hacl.Impl.PKCS11.DeviceModule
+
+open FStar.HyperStack.All
+open FStar.HyperStack
+module ST = FStar.HyperStack.ST
+
+open Lib.RawIntTypes
+open LowStar.Buffer
+
+
+val isAttributeEC_PARAMCorrect: d: device ->  a: attribute {CKA_EC_PARAMS? a} -> Stack (((e: exception_t) & (_HACL_Curve_ID)))
+  (requires fun h -> True)
+  (ensures fun h0 _ h1 -> True)
+
+let isAttributeEC_PARAMCorrect d a = 
+  let ulCount = CKA_EC_PARAMS?.ulValueLen a in 
+  let (|exc, curveIdentifier|) = parseEC_ANSI_962 (CKA_EC_PARAMS?.ulValueLen a) (CKA_EC_PARAMS?.pValue a) in  
+  match exc with 
+  |CKR_OK -> 
+    let curveSupported = isCurveSupported d curveIdentifier in 
+    match curveSupported with 
+      |true -> (|CKR_OK, curveIdentifier|)
+      |false -> (|CKR_CURVE_NOT_SUPPORTED, curveIdentifier|)
+  | _ -> (|exc, curveIdentifier|)
+  
+
+
+val checkAttributes: ulCount: size_t -> pTemplate: buffer attribute{length pTemplate = uint_v ulCount} -> Stack unit
+  (requires fun h -> live h pTemplate)
+  (ensures fun h0 _ h1 -> True)
+
+let checkAttributes ulCount pTemplate = 
+  push_frame();
+  [@inline_let]
+  let okException = CKR_OK in 
+  let bTest = LowStar.Buffer.alloca okException (normalize_term 1ul) in  
+  C.Loops.for 0ul ulCount (fun h i -> True) (fun i ->  isAttributeReadOnlyBuffer (index pTemplate i) bTest);
+  pop_frame()
